Modal/modal/sound_complete/M_upnbhd.lean
@@ -4,18 +4,21 @@ import Modal.modal.proof_systems.E_proof
 
 namespace Modal.SoundComplete.M_UpNbhd
 
-open Modal.ProofSystems Modal.Models
+open Modal.ProofSystems Modal.Models.Nbhd
 
+def upward_closed (f : Frame) : Prop :=
+  ∀ w : f.world, ∀ X Y : Set f.world, X ∈ f.nbhd w → X ⊆ Y → Y ∈ f.nbhd w
 
-def is_upclosed : Nbhd.Frame → Prop :=
-  fun f => ∀ w (X Y : Set f.world), X ∈ f.nbhd w → X ⊆ Y → Y ∈ f.nbhd w
+def upward_closed_semantics {Atom : Type} : Logic.Semantics (Formula Atom) :=
+  { model := { m : Model Atom // upward_closed m.frame },
+    satisfies := fun m φ => model_sat m.val φ }
 
 theorem is_sound_strong (Atom : Type) :
-    Logic.is_sound_strong (E.proof_system Atom) (@Nbhd.semantics Atom is_upclosed) :=
+    Logic.is_sound_strong (E.proof_system Atom) upward_closed_semantics :=
   by admit
 
 theorem is_complete_weak (Atom : Type) :
-    Logic.is_complete_weak (E.proof_system Atom) (@Nbhd.semantics Atom is_upclosed) :=
+    Logic.is_complete_weak (E.proof_system Atom) upward_closed_semantics :=
   by admit
 -- M is not strongly complete wrt upclosed neighbourhood models
 
