Modal/modal/sound_complete/E_nbhd.lean
@@ -6,15 +6,12 @@ namespace Modal.SoundComplete.E_Nbhd
 
 open Modal.ProofSystems Modal.Models
 
-
-def all_frames : Nbhd.Frame → Prop := fun _ => True
-
 theorem is_sound_strong (Atom : Type) :
-    Logic.is_sound_strong (E.proof_system Atom) (@Nbhd.semantics Atom all_frames) :=
+    Logic.is_sound_strong (E.proof_system Atom) Nbhd.semantics :=
   by admit
 
 theorem is_complete_weak (Atom : Type) :
-    Logic.is_complete_weak (E.proof_system Atom) (@Nbhd.semantics Atom all_frames) :=
+    Logic.is_complete_weak (E.proof_system Atom) Nbhd.semantics :=
   by admit
 -- E is not strongly complete wrt neighborhood models
 
